\subsubsection*{a)}
\begin{align*}
f&= \left(AG(Error \Rightarrow E(Error U \neg Battery))\right) \wedge \left( \neg AF Acrive\right)\\
&\equiv \left(AG(Error \Rightarrow E(Error U \neg Battery))\right) \wedge \left( \neg \neg EG( \neg Acrive)\right)\\
&\equiv \left(AG(Error \Rightarrow E(Error U \neg Battery))\right) \wedge \left( EG( \neg Acrive)\right)\\
&\equiv \left(\neg EF (\neg(Error \Rightarrow E(Error U \neg Battery)))\right) \wedge \left( EG( \neg Acrive)\right)\\
&\equiv \left(\neg EF (\neg(\neg Error \vee E(Error U \neg Battery)))\right) \wedge \left( EG( \neg Acrive)\right)\\
&\equiv \neg\left(\neg \neg EF (\neg(\neg Error \vee E(Error U \neg Battery)))\right) \vee \left(\neg EG( \neg Acrive)\right)\\
&\equiv \neg\left(EF (\neg(\neg Error \vee E(Error U \neg Battery)))\right) \vee \left(\neg EG( \neg Acrive)\right)\\
&\equiv \neg\left(E (trueU (\neg(\neg Error \vee E(Error U \neg Battery))))\right) \vee \left(\neg EG( \neg Acrive)\right)\\
\end{align*}

Man dr√∂selt die Formel durch Rekursion auf, wie soll man das jetzt aufschreiben??

\subsubsection*{b)}
\begin{align*}
g&=	AGEF(Active)\\
&\equiv\neg EF \neg EF (Active)\\
&\equiv\neg E(true U (\neg E(trueU (Active)))\\
\end{align*}



